theories/simulations/msim/MSim.v
@@ -1,49 +1,6 @@
 Require Import Common.
 From iris.proofmode Require Import proofmode.
-Require Import LSim Sandbox Mod.
-
-Variant contextuality : Type := 
-| open 
-| closed.
-
-Notation ist_type Σ := (nat → alist key Any.t → alist key Any.t → iProp Σ).
-Notation retr_type Σ Rs Rt := (nat → alist key Any.t * Rs → alist key Any.t * Rt → iProp Σ).
-Notation msim_type Σ Rs Rt := (bool → bool → nat → alist key Any.t * itree crisE Rs → alist key Any.t * itree crisE Rt → Σ → Prop).
-
-Section IST.
-
-  Context `{Σ: GRA}.
-
-  Definition Ist_monotone (Ist: ist_type Σ) : Prop :=
-    ∀ nths nths' (LE : nths <= nths') st_src st_tgt,
-      Ist nths st_src st_tgt ⊢ Ist nths' st_src st_tgt.
-
-  Definition IstProd (IstL IstR : ist_type Σ) :=
-  fun nths (st_src st_tgt : alist key Any.t) =>
-    (∃ st_srcL st_tgtL st_srcR st_tgtR,
-     ⌜st_src = st_srcL ++ st_srcR /\ st_tgt = st_tgtL ++ st_tgtR⌝ ∗
-     IstL nths st_srcL st_tgtL ∗ IstR nths st_srcR st_tgtR)%I.
-
-  Definition IstSB scopes (Ist : ist_type Σ) :=
-    fun nths st_src st_tgt =>
-      (⌜incl (Mod.state_scopes st_src) scopes ∧
-         incl (Mod.state_scopes st_tgt) scopes⌝
-           ∗ Ist nths st_src st_tgt)%I.
-
-  Definition IstEq : ist_type Σ :=
-    (fun _ st_src st_tgt => ⌜st_src = st_tgt⌝)%I.
-
-  Definition ist_with_eq (Ist : ist_type Σ) {R} :=
-    fun nths '(st_src, v_src) '(st_tgt, v_tgt) =>
-      (⌜v_src = (v_tgt: R)⌝ ∗ Ist nths st_src st_tgt)%I.
-
-  Definition IstTrue : ist_type Σ
-    := λ _ _ _, True%I.
-
-  Definition IstFalse : ist_type Σ
-    := λ _ _ _, False%I.
-
-End IST.
+Require Import Sandbox Mod LSim MSimCommon.
 
 Section MSIM.
 
