theories/cancellation/MInlineIntro.v
@@ -1,15 +1,18 @@
 Require Import Common.
 From iris.proofmode Require Import proofmode.
 Require Import SModTr SMod Mod Tactics.
-Require Import ISim ISimInit CtxRefine CtxRefineFacts ClosedAdequacy.
+Require Import ISim ISimFacts CtxRefine CtxRefineFacts ClosedAdequacy.
 Require Import MInline.
 
 Set Implicit Arguments.
 
-Lemma inline_intro `{Σ: GRA} md P
+Section INLINE.
+Context `{_crisG: !crisG Γ Σ α β τ _S _I}.
+
+Lemma inline_intro md P
   :
   refines (MInline.inline md, P) (md, P).
-Proof.
+Proof using.
   eapply closed_adequacy_emp. clear P.
 
   cut (∀ f (WF: Mod.wf md) (SCP: incl f.1.2 md.(Mod.scopes)),
@@ -29,7 +32,7 @@ Proof.
     { ii. rewrite alist_find_map_snd in FIND.
       destruct (alist_find fn (Mod.fnsems md)) eqn:FINDT; ss.
       inv FIND. esplits; eauto.
-      ii. iIntros "H". iAssert (⌜st_src = st_tgt⌝)%I as "%EQ".
+      ii. iIntros "H I". iAssert (⌜st_src = st_tgt⌝)%I as "%EQ".
       { destruct fn; iDestruct "H" as "%"; des; subst; et. }
       subst. iApply isim_mono; cycle 1.
       - iApply H; et.
@@ -39,7 +42,7 @@ Proof.
     }
   }
 
-  ii. iIntros "%". subst.
+  ii. iIntros "% I". subst. iStopProof.
   destruct f as [[[img msk] scp] bd].
   do 2 (rewrite /SB.sandbox_body; s).
 
@@ -47,7 +50,7 @@ Proof.
   generalize (bd arg) as it. i.
   ss. clear bd arg NODD NODS. rename st_tgt into st.
 
-  iStopProof. revert it.
+  revert it.
   combine_quant st.
   combine_quant pt.
   combine_quant ps.
@@ -60,7 +63,7 @@ Proof.
   eapply isim_coind. i.
   destruct a as [scp [SCP [nths [img [msk [ps [pt [st it]]]]]]]]; s.
   destruct_quant.
-  iIntros "(_ & #CIH)".
+  iIntros "(I & #CIH)".
 
   assert (CASE := case_itrH it); des; subst.
   - rewrite SBRed.ret MIRed.ret. step. eauto.
@@ -86,7 +89,8 @@ Proof.
       s. ired. rewrite /SB.sandbox_body. s.
 
       rewrite MIRed.bind SBRed.bind.
-      iApply isim_bind; iSplitL.
+      iPoseProof (winv_split_empty with "[I]") as "[I I']"; et.
+      iApply isim_bind. iSplitL "I".
       - by_coind "CIH"; et.
         iPureIntro. ii. exploit Mod.well_scoped_fns; et.
         rewrite /fnsems_scopes. erewrite FIND. et.
@@ -140,3 +144,5 @@ Proof.
     + rewrite SBRed.bind SBRed.io MIRed.core.
       step. steps_l. by_coind "CIH"; et.
 (*SLOW*)Qed.
+
+End INLINE.
